Shapeview.v
@@ -1,0 +1,26 @@
+Require Import MLTTTyping LogicalRelation.
+
+Check LRPi.
+
+Inductive ShapeView Γ (l l' : TypeLevel) : 
+    forall A B, [Γ ||-< l | A] -> [Γ ||-< l' | B] -> Type 
+:=
+    | SVU {la l_a Γa lb l_b Γb} :
+        ShapeView Γ l l' U U 
+         (LRU_ Γa la l_a)
+         (LRU_ Γb lb l_b)
+
+    | SVne {A B} neA neB :
+        ShapeView Γ l l' A B
+        (LRne_ _ _ neA)
+        (LRne_ _ _ neB)
+
+    | SVPi {A B} Π0A Π0B Π1A Π1B:
+        ShapeView Γ l l' A B
+        (LRPi_ _ _ Π0A Π1A)
+        (LRPi_ _ _ Π0B Π1B)
+         
+    | SVemb01 {A B p q} (leq : l = one) :
+      ShapeView Γ zero l' A B p q ->
+      ShapeView Γ l l' A B (LREmb_ _  (LESubst leq) p) q   
+          . 
