Symmetry.v
@@ -1,0 +1,12 @@
+Require Import Untyped MLTTTyping LogicalRelation Properties Reduction LRInduction.
+
+Set Universe Polymorphism.
+
+Definition Sym0 {Γ A B l l'} (ha : [Γ ||-< zero | A]) (hb : [Γ ||-< zero | B]) :
+    [Γ ||-< zero | A ≅ B | ha ] ->
+    [Γ ||-< zero | B ≅ A | hb ].
+Proof.
+    intros.
+    destruct ha.
+    destruct hb.
+    destruct valid.
